vera/VerilogToSMTCorrect.v
@@ -10,15 +10,16 @@ Import CombinationalOnly.
 From vera Require Import Bitvector.
 Import RawXBV(bit(..)).
 
-From Coq Require List.
-From Coq Require String.
-From Coq Require Import Logic.ProofIrrelevance.
-From Coq Require Import NArith.
-
 From ExtLib Require Import Structures.MonadExc.
 From ExtLib Require Import Structures.MonadState.
 From ExtLib Require Import Structures.Monads.
 From ExtLib Require Import Structures.Functor.
+
+From Coq Require List.
+From Coq Require String.
+From Coq Require Import Logic.ProofIrrelevance.
+From Coq Require Import NArith.
+From Coq Require Import PeanoNat.
 
 From Equations Require Import Equations.
 
@@ -453,19 +454,40 @@ Corollary cast_from_to_zextn_inv ρ (from to : N) bv_from result t :
   result = Some (SMTLib.Value_BitVec _ (BV.bv_concat (BV.zeros (to - from)) bv_from)).
 Admitted.
 
-Definition xbv_to_N {w} (bv : XBV.xbv w) : option N :=
-  option_map BV.to_N (XBV.to_bv bv).
+Lemma to_N_from_bv n (b : BV.bitvector n) : XBV.to_N (XBV.from_bv b) = Some (BV.to_N b).
+Proof. unfold XBV.to_N. now rewrite XBV.xbv_bv_inverse. Qed.
+
+Lemma bv_to_N_max_bound n (b : BV.bitvector n) : (BV.to_N b < 2 ^ n)%N.
+Proof.
+  intros.
+  unfold BV.to_N, RawBV.to_N, RawBV.size.
+  destruct b. simpl. subst.
+  unfold RawBV.size in *.
+  replace (2 ^ N.of_nat (length bv))%N with (N.of_nat (2 ^ length bv))
+    by now rewrite Nat2N.inj_pow.
+  enough (RawBV.list2nat_be bv < 2 ^ (length bv)) by lia.
+  induction bv; intros; try crush.
+  cbn in *. rewrite ! RawBV._list2nat_be_arith in *.
+  crush.
+Qed.
 
 Lemma statically_in_bounds_max_bound {w} max_bound e regs (xbv : XBV.xbv w) val :
   statically_in_bounds max_bound e ->
   eval_expr regs e = Some xbv ->
-  xbv_to_N xbv = Some val ->
+  XBV.to_N xbv = Some val ->
   (val < max_bound)%N.
 Proof.
+  unfold statically_in_bounds, static_value.
   intros Hinbounds Heval HtoN.
   inv Hinbounds.
-  - destruct (static_value e); cbn in *.
-
+  - destruct e; try crush.
+    simp eval_expr in Heval. inv Heval.
+    rewrite to_N_from_bv in HtoN. inv HtoN.
+    crush.
+  - unfold XBV.to_N in *. destruct (XBV.to_bv xbv); try discriminate. inv HtoN.
+    enough (BV.to_N b < 2 ^ w)%N by lia.
+    apply bv_to_N_max_bound.
+Qed.
 
 Lemma expr_to_smt_correct {w} (vars : StrFunMap.t smt_var_info) (expr : Verilog.expression w) :
   forall t tag (m : VerilogSMTBijection.t) regs ρ xbv bv,
@@ -584,12 +606,18 @@ Proof.
         erewrite cast_from_to_zextn in *; try crush.
         some_inv; now rewrite BV.bv_zextn_to_N.
       }
-
+      unfold XBV.bitOf, RawXBV.bitOf.
+      admit.
       (* TODO: select_bit with the original bitvectors is the same as select bit on the zero-extended values. *)
       (* TODO: Should be provable as long as the index is in-bounds. See below *)
-      admit.
-    + admit.
-      (* TODO: Index is in bounds. Does not hold, not sure how to handle. *)
+    + clear E. eapply statically_in_bounds_max_bound in s; eauto using to_N_from_bv.
+      replace (BV.to_N bv4) with (BV.to_N bv0); cycle 1. {
+        erewrite cast_from_to_zextn in *; try crush.
+        some_inv; now rewrite BV.bv_zextn_to_N.
+      }
+      enough (Verilog.expr_type vec <= w)%N by lia.
+      replace w with (N.max (Verilog.expr_type vec) (Verilog.expr_type idx)) by admit.
+      lia.
   - (* Concatenation *)
     expr_begin_tac.
     apply verilog_smt_match_to_bv.
